AltTraces.v
@@ -1,10 +1,8 @@
-Require Import List.
+Require Export Derivations Subformulas FLSubformulas.
+
 Import ListNotations.
 
-Require Import Debruijn Derivations Occurrences FLSubformulas.
-Local Open Scope eqb_scope.
-Local Open Scope form.
-
+Module Inductive_attempt.
 
 (** DEFINITION *)
 
@@ -12,50 +10,50 @@ Local Open Scope form.
 
 Definition FPathType := list sequent.
 
-Inductive preFPath : FPathType -> derivation -> Prop :=
- | Lf s s' ls R: s = (oseq_forget s') -> preFPath [s] (ORule ls R s' []) 
- | COne d t R ls s s': 
-                          preFPath t d -> s' = oseq_forget s -> preFPath (s'::t) (ORule ls R s [d])
- | CLeft d d' R ls t s s': 
-                          preFPath t d -> s' = oseq_forget s -> preFPath (s'::t) (ORule ls R s [d;d'])
- | CRight d d' R ls t s s': 
-                          preFPath t d -> s' = oseq_forget s -> preFPath (s'::t) (ORule ls R s [d';d]).
+Inductive preFPath : FPathType -> derivation -> nat -> Prop :=
+ | CLeaf s s' ls n: s = (oseq_forget s') -> preFPath [s] (ORule ls (BackEdge n) s' []) n 
+ | COne d t R ls s s' n: 
+                          preFPath t d n -> s' = oseq_forget s -> preFPath (s'::t) (ORule ls R s [d]) n
+ | CLeft d d' R ls t s s' n: 
+                          preFPath t d n -> s' = oseq_forget s -> preFPath (s'::t) (ORule ls R s [d;d']) n
+ | CRight d d' R ls t s s' n: 
+                          preFPath t d n -> s' = oseq_forget s -> preFPath (s'::t) (ORule ls R s [d';d]) n.
 
-Definition preFPathNode (t:FPathType)(d:derivation)(a:address) :=
+Definition preFPathNode t d n a :=
   match subderiv d a with
   | None       => False
-  | Some d'  => preFPath t d'
+  | Some d'  => preFPath t d' n
   end.
 
-Definition FPath (t:FPathType)(d:derivation)(a:address) : Prop := (Valid d) /\ (preFPathNode t d a). 
+Definition FPath t d n a : Prop := (Valid d) /\ (preFPathNode t d n a). 
 
 (** FInite Traces *)
 
 Definition FTraceType := list (formula*sequent).
 
-Inductive preFTrace : FTraceType -> derivation -> Prop :=
- | Leaf f s s' ls R: s = (oseq_forget s') -> In f s -> preFTrace [(f,s)] (ORule ls R s' []) 
- | ConsOne d t R ls s0 s s' f1 f2: 
-                          preFTrace ((f1,s0)::t) d -> s' = oseq_forget s 
+Inductive preFTrace : FTraceType -> derivation -> nat -> Prop :=
+ | Leaf f s s' ls n: s = (oseq_forget s') -> In f s -> preFTrace [(f,s)] (ORule ls (BackEdge n) s' []) n 
+ | ConsOne d t R ls s0 s s' f1 f2 n: 
+                          preFTrace ((f1,s0)::t) d n -> s' = oseq_forget s 
                           -> In f2 s' -> In f1 (FL f2) 
-                          -> preFTrace ((f2,s')::(f1,s0)::t) (ORule ls R s [d])
- | ConsLeft d d' t R ls s0 s s' f1 f2: 
-                          preFTrace ((f1,s0)::t) d -> s' = oseq_forget s 
+                          -> preFTrace ((f2,s')::(f1,s0)::t) (ORule ls R s [d]) n
+ | ConsLeft d d' t R ls s0 s s' f1 f2 n: 
+                          preFTrace ((f1,s0)::t) d n -> s' = oseq_forget s 
                           -> In f2 s' -> In f1 (FL f2) 
-                          -> preFTrace ((f2,s')::(f1,s0)::t) (ORule ls R s [d;d'])
- | ConsRight d d' t R ls s0 s s' f1 f2: 
-                          preFTrace ((f1,s0)::t) d -> s' = oseq_forget s 
+                          -> preFTrace ((f2,s')::(f1,s0)::t) (ORule ls R s [d;d']) n
+ | ConsRight d d' t R ls s0 s s' f1 f2 n: 
+                          preFTrace ((f1,s0)::t) d n -> s' = oseq_forget s 
                           -> In f2 s' -> In f1 (FL f2) 
-                          -> preFTrace ((f2,s')::(f1,s0)::t) (ORule ls R s [d';d])
+                          -> preFTrace ((f2,s')::(f1,s0)::t) (ORule ls R s [d';d]) n
                         .
 
-Definition preFTraceNode (t:FTraceType)(d:derivation)(a:address) :=
+Definition preFTraceNode t d n a :=
   match subderiv d a with
   | None       => False
-  | Some d'  => preFTrace t d'
+  | Some d'  => preFTrace t d' n
   end.
 
-Definition FTrace (t:FTraceType)(d:derivation)(a:address) : Prop := (Valid d) /\ (preFTraceNode t d a). 
+Definition FTrace t d n a : Prop := (Valid d) /\ (preFTraceNode t d n a). 
 
 
 (** Link between both*)
@@ -65,12 +63,14 @@ Definition IsFTrace (t:FTraceType)(p:FPathType): Prop := map snd t = p.
 
 (** Example *)
 
+Local Open Scope form.
+
 Definition FTrace_example: FTraceType := 
   [( ν (%0)⊕(%0), ⊦ [(ν (%0)⊕(%0))]);
    (((ν (%0)⊕(%0)) ⊕ (ν (%0)⊕(%0))), ⊦ [((ν (%0)⊕(%0)) ⊕ (ν (%0)⊕(%0)))] );
    (ν (%0)⊕(%0), ⊦ [ν (%0)⊕(%0)] )].
 
-Lemma FTrace_example_lemma : FTrace FTrace_example oderiv_example' [].
+Lemma FTrace_example_lemma : FTrace FTrace_example oderiv_example' 2 [].
 Proof.
   split;
   repeat (constructor; simpl; intuition).
@@ -94,26 +94,135 @@ Definition TraceRepeat (t:FTraceType) := (fun (n:nat) => t).
 
 Definition Trace_Example := TraceRepeat FTrace_example.
 
+End Inductive_attempt.
 
 
+(** Fixpoint version *)
+
+Module fixpoint_attempt.
+
+(** DEFINITION *)
+
+(** Finite Paths *)
+
+Definition FPathType := list sequent.
+
+Fixpoint preFPath p d n: Prop :=
+  let '(ORule ls R s ld) := d in 
+  match p with
+  | []       => False
+  | s'::p' => s' = (oseq_forget s) /\
+                  match ld, R, p' with
+                  | [], BackEdge n', [] =>  n = n' 
+                  | [d'], _, _                  => preFPath p' d' n
+                  | [d1;d2], _, _           => preFPath p' d1 n \/ preFPath p' d2 n
+                  | _, _, _                     => False
+                  end
+  end.
+
+Definition preFPathNode t d n a :=
+  match subderiv d a with
+  | None       => False
+  | Some d'  => preFPath t d' n
+  end.
+
+Definition FPath t d n a : Prop := (Valid d) /\ (preFPathNode t d n a). 
+
+(** FInite Traces *)
+
+Definition FTraceType := list (formula*sequent).
+
+Fixpoint preFTrace p d n: Prop :=
+  let '(ORule ls R s ld) := d in 
+  match p with
+  | []       => False
+  | (f1,s')::p' => s' = (oseq_forget s) /\
+                            match ld, R, p' with
+                            | [], BackEdge n', [] =>  (In f1 s') /\ (n = n') 
+                            | [d'], _, (f2,_)::p'' => In f1 s' /\ In f2 (FL f1) /\ preFTrace p' d' n
+                            | [d1;d2], _, (f2, _)::p''  => In f1 s' /\ In f2 (FL f1) /\ (preFTrace p' d1 n \/ preFTrace p' d2 n)
+                            | _, _, _                     => False
+                            end
+  end.
+
+Definition preFTraceNode t d n a :=
+  match subderiv d a with
+  | None       => False
+  | Some d'  => preFTrace t d' n
+  end.
+
+Definition FTrace t d n a : Prop := (Valid d) /\ (preFTraceNode t d n a). 
 
 
+(** Link between both*)
 
+Definition IsFTrace (t:FTraceType)(p:FPathType): Prop := map snd t = p. 
+
+
+(** Example *)
+
+Local Open Scope form.
+
+Definition FTrace_example: FTraceType := 
+  [( ν (%0)⊕(%0), ⊦ [(ν (%0)⊕(%0))]);
+   (((ν (%0)⊕(%0)) ⊕ (ν (%0)⊕(%0))), ⊦ [((ν (%0)⊕(%0)) ⊕ (ν (%0)⊕(%0)))] );
+   (ν (%0)⊕(%0), ⊦ [ν (%0)⊕(%0)] )].
+
+Lemma FTrace_example_lemma : FTrace FTrace_example oderiv_example' 2 [].
+Proof.
+  split.
+  - repeat (constructor; simpl; intuition).
+  - cbn; intuition.
+Qed.
+
+(** Infinite Paths/Traces *)
+
+Definition PathType: Type := nat -> FPathType.
+
+Definition TraceType: Type := nat -> FTraceType.
+
+(** Link between both *)
+
+Definition IsTrace (T:TraceType)(P:PathType): Prop := forall n, map snd (T n) = P n. 
+
+(** Example *)
+
+Definition PathRepeat (t:FPathType) := (fun (n:nat) => t).
+
+Definition TraceRepeat (t:FTraceType) := (fun (n:nat) => t).
+
+Definition Trace_Example := TraceRepeat FTrace_example.
 
 (** PATH & TRACE VALIDITY *)
 
+
 Local Open Scope eqb_scope.
 
-(** Access to the last rule used in [d] (following address [a] in [d]) *)
-
-Definition last_trace_rule (d:derivation)(a:address) : option rule_kind :=
-  match subderiv d a with
-  | None => None
-  | Some d' => let '(ORule ls R s ld) := d' in match ld with 
-                                                                   | [] => Some R
-                                                                   | _ => None
-                                                                   end
-  end.
-
 (** Linking condition between Stream's elements *)
+
+Definition Path (P:PathType)(d:derivation): Prop := 
+  exists a m, FPath (P 0) d m a /\
+  forall n, exists an aSn mn mSn, 
+    (FPath (P n) d mn an) /\ (npop mn an = Some aSn) /\ (FPath (P (S n)) d mSn aSn).
+
+
+Definition Trace (P:TraceType)(d:derivation): Prop := 
+  exists a m, FTrace (P 0) d m a /\
+  forall n, exists an aSn mn mSn, 
+    (FTrace (P n) d mn an) /\ (npop mn an = Some aSn) /\ (FTrace (P (S n)) d mSn aSn).
+
+(* Very hard to work with inductive notions. *)
+
+End fixpoint_attempt.
+
+
+
+
+
+
+
+
+
+
+
 
